details

src/tls/Handshake.fst
@@ -36,7 +36,7 @@ module Nego = Negotiation
 open Negotiation // regretfully: too many record fields.
 
 let hashSize = Hashing.Spec.tagLen
-
+ 
 //<expose for TestClient> CF: temporarily broken; such tests should be coded against HS submodules.
 // TODO restore unit tests as in TestClient
 
@@ -52,7 +52,7 @@ inline_for_extraction let hs_debug = false
 val trace: s:string -> ST unit 
   (requires (fun _ -> True))
   (ensures (fun h0 _ h1 -> h0 == h1))
-let trace s = if hs_debug then IO.print_string ^"HS| "^s^"\n"
+let trace s = if hs_debug then IO.print_string ("HS| "^s^"\n")
 
 
 (* Returns [c] if [c] is within the range of acceptable versions for [cfg],
@@ -244,48 +244,6 @@ let in_next_keys (r:incoming) = InAck? r && InAck?.next_keys r
 let in_complete (r:incoming)  = InAck? r && InAck?.complete r
 
 
-(* ---------------- signature stuff, to be moved (at least) to Nego -------------------- *)
-
-// deep subtyping...
-let optHashAlg_prime_is_optHashAlg: result hashAlg' -> Tot (result TLSConstants.hashAlg) =
-  function
-  | Error z -> Error z
-  | Correct h -> Correct h
-let sigHashAlg_is_tuple_sig_hash: sigHashAlg -> Tot (sigAlg * TLSConstants.hashAlg) =
-  function | a,b -> a,b
-let rec list_sigHashAlg_is_list_tuple_sig_hash: list sigHashAlg -> Tot (list (TLSConstants.sigAlg * TLSConstants.hashAlg)) =
-  function
-  | [] -> []
-  | hd::tl -> (sigHashAlg_is_tuple_sig_hash hd) :: (list_sigHashAlg_is_list_tuple_sig_hash tl)
-
-val to_be_signed: pv:protocolVersion -> role -> csr:option bytes{None? csr <==> pv = TLS_1p3} -> bytes -> Tot bytes
-let to_be_signed pv role csr tbs =
-  match pv, csr with
-  | TLS_1p3, None ->
-    let pad = abytes (String.make 64 (Char.char_of_int 32)) in
-    let ctx =
-      match role with
-      | Server -> "TLS 1.3, server CertificateVerify"
-      | Client -> "TLS 1.3, client CertificateVerify"
-    in
-    pad @| (abytes ctx) @| (abyte 0z) @| tbs
-  | _, Some csr -> csr @| tbs
-
-val sigHashAlg_of_ske: bytes -> Tot (option (sigHashAlg * bytes))
-let sigHashAlg_of_ske signature =
-  if length signature > 4 then
-   let h, sa, sigv = split2 signature 1 1 in
-   match vlsplit 2 sigv with
-   | Correct (sigv, eof) ->
-     begin
-     match length eof, parseSigAlg sa, optHashAlg_prime_is_optHashAlg (parseHashAlg h) with
-     | 0, Correct sa, Correct (Hash h) -> Some ((sa,Hash h), sigv)
-     | _, _, _ -> None
-     end
-   | Error _ -> None
-  else None
-
-
 // factored out; indexing to be reviewed
 let register hs keys =
     let ep = //? we don't have a full index yet for the epoch; reuse the one for keys??
@@ -416,65 +374,31 @@ let client_ServerHelloDone hs c ske ocr =
         g in
       let msg = ClientKeyExchange ({cke_kex_c = kex_c_of_dh_key #g gx}) in
       let digestClientKeyExchange = Handshake.Log.send_tag hs.log msg  in
+      ( match ocr with
+        | None -> ()
+        | Some cr ->
+            let cc = {crt_chain = []} in // TODO
+            Handshake.Log.send hs.log (Certificate cc));
 
-    (* here are the checks we were doing before; now hopefully in Nego:
-    let valid_chain = hs.cfg.check_peer_certificate => Cert.validate_chain c.crt_chain true cfg.peer_name cfg.ca_file in
-    if not valid_chain then Error (AD_certificate_unknown_fatal, perror __SOURCE_FILE__ __LINE__ "Certificate validation failure")    else
-      let ske_tbs = kex_s_to_bytes ske.ske_kex_s in
-      let Some cs_sigalg = n.n_sigAlg in
-      let sigalgs = n.n_extensions.ne_signature_algorithms in
-      match sigHashAlg_of_ske ske.ske_sig with
-      | None -> Error (AD_decode_error, perror __SOURCE_FILE__ __LINE__ "Failed to parse SKE message")
-      | Some ((sa,h),sigv) ->
-            let algs: list sigHashAlg =
-              match sigalgs with
-              | Some l -> l
-              | None -> [(cs_sigalg, Hash Hashing.Spec.SHA1)] in
-            if not (List.Tot.existsb (fun (xs,xh) -> (xs = sa && xh = h)) algs)
-            then Error (AD_handshake_failure, perror __SOURCE_FILE__ __LINE__ "Signature algorithm negotiation failed")
-            else
-              let a = Signature.Use (fun _ -> true) sa [h] false false in
-              let csr = (n.n_client_random @| n.n_server_random) in
-              let ems = n.n_extensions.ne_extended_ms in
-              let tbs = to_be_signed n.n_protocol_version Server (Some csr) ske_tbs in
-              match Signature.get_chain_public_key #a c.crt_chain with
-              | None -> Error (AD_handshake_failure, perror __SOURCE_FILE__ __LINE__ "failed to get public key from chain") )
-              | Some pk ->
-                   let valid_signature = Signature.verify #a h pk tbs sigv in
-                   // debug_print("tbs = " ^ (Platform.Bytes.print_bytes tbs) ^ "\n");
-                   debug_print("Signature validation status = " ^ (if valid then "OK" else "FAIL") ^ "\n");
-                   if not valid_signature then Error (AD_handshake_failure, perror __SOURCE_FILE__ __LINE__ "failed to check SKE signature")
-                   else
-                     match ske.ske_kex_s with
-                     | KEX_S_RSA _ -> Error (AD_handshake_failure, perror __SOURCE_FILE__ __LINE__ "only support ECDHE/DHE SKE") )
-                     | KEX_S_DHE (| g, gy |) ->
-                     *)
+      let (| g, _ |) = Some?.v (mode.Nego.n_server_share) in // already set in KS
+      let gx =
+        KeySchedule.ks_client_12_full_dh hs.ks
+        mode.Nego.n_server_random
+        mode.Nego.n_protocol_version
+        mode.Nego.n_cipher_suite
+        mode.Nego.n_extensions.ne_extended_ms // a flag controlling the use of ems
+        g in
+      let msg = ClientKeyExchange ({cke_kex_c = kex_c_of_dh_key #g gx}) in
+      let digestClientKeyExchange = Handshake.Log.send_tag hs.log msg  in
 
-                       ( match ocr with
-                         | None -> ()
-                         | Some cr ->
-                             let cc = {crt_chain = []} in // TODO
-                             Handshake.Log.send hs.log (Certificate cc));
+      let cfin_key, app_keys = KeySchedule.ks_client_12_set_session_hash hs.ks digestClientKeyExchange in
+      register hs app_keys;
+      // we send CCS then Finished;  we will use the new keys only after CCS
 
-                       let (| g, _ |) = Some?.v (mode.Nego.n_server_share) in // already set in KS
-                       let gx =
-                         KeySchedule.ks_client_12_full_dh hs.ks
-                         mode.Nego.n_server_random
-                         mode.Nego.n_protocol_version
-                         mode.Nego.n_cipher_suite
-                         mode.Nego.n_extensions.ne_extended_ms // a flag controlling the use of ems
-                         g in
-                       let msg = ClientKeyExchange ({cke_kex_c = kex_c_of_dh_key #g gx}) in
-                       let digestClientKeyExchange = Handshake.Log.send_tag hs.log msg  in
-
-                       let cfin_key, app_keys = KeySchedule.ks_client_12_set_session_hash hs.ks digestClientKeyExchange in
-                       register hs app_keys;
-                       // we send CCS then Finished;  we will use the new keys only after CCS
-
-                       let cvd = TLSPRF.verifyData (mode.Nego.n_protocol_version,mode.Nego.n_cipher_suite) cfin_key Client digestClientKeyExchange in
-                       let digestClientFinished = Handshake.Log.send_CCS_tag hs.log (Finished ({fin_vd = cvd})) false in
-                       hs.state := C_Wait_CCS2 digestClientFinished;
-                       InAck false false)
+      let cvd = TLSPRF.verifyData (mode.Nego.n_protocol_version,mode.Nego.n_cipher_suite) cfin_key Client digestClientKeyExchange in
+      let digestClientFinished = Handshake.Log.send_CCS_tag hs.log (Finished ({fin_vd = cvd})) false in
+      hs.state := C_Wait_CCS2 digestClientFinished;
+      InAck false false)
 
 #set-options "--lax"
 (* receive EncryptedExtension...ServerFinished for TLS 1.3, roughly mirroring client_ServerHelloDone *)
